verif/verif_gotokey.v
@@ -17,13 +17,173 @@ Require Import btrees_sep.
 Require Import btrees_spec.
 Require Import verif_findindex.
 Require Import verif_isnodeparent.
+Require Import verif_movetokey.
 
 Lemma body_AscendToParent: semax_body Vprog Gprog f_AscendToParent AscendToParent_spec.
 Proof.
   start_function.
+  destruct r as [root prel].
+  pose (r:=(root,prel)).
+  unfold cursor_rep. Intros anc_end. Intros idx_end.
+  forward.                      (* t'4=cursor->level *)
+  forward_if.
+  - forward.                    (* return *)
+    entailer!. destruct c.
+    + simpl. unfold cursor_rep.
+      Exists anc_end. Exists idx_end. simpl. cancel.
+    + rewrite Zlength_cons in H3. rewrite Zsuccminusone in H3.
+      apply partial_complete_length in H; auto. rewrite Zlength_cons in H. rewrite Zsuccminusone in H.
+      apply (f_equal Int.unsigned) in H3. rewrite Int.unsigned_repr in H3; try rep_omega.
+      rewrite Int.unsigned_repr in H3; try rep_omega. destruct c as [|[n i] c'].
+      * simpl. destruct p. simpl. unfold cursor_rep.
+        Exists anc_end. Exists idx_end. cancel.
+      * rewrite Zlength_cons in H3. rep_omega.
+  - forward.                    (* skip *)
+    forward_call(r,c,pc).       (* t'1=currnode(cursor) *)
+    { unfold r. unfold cursor_rep. Exists anc_end. Exists idx_end. cancel.
+      change_compspecs CompSpecs. cancel. }
+    destruct c as [|[n i] c'] eqn:HC.
+    { destruct H. inv H. destruct H5. inv H. inv H. inv H4. } simpl.
+    assert(SUBNODE: subnode n root).
+    { destruct H.
+      - inv H. apply partial_cursor_subnode in H4. simpl in H4. auto.
+      - inv H. apply complete_cursor_subnode in H4. simpl in H4. auto. }
+    forward_call(n,key).          (* t'2=isNodeParent(t'1,key) *)
+    { apply subnode_rep in SUBNODE. rewrite SUBNODE. cancel. }
+    gather_SEP 0 3. replace_SEP 0 (btnode_rep root).
+    { entailer!. apply wand_frame_elim. }
+    forward_if.                 (* if t'2=1 *)
+    + forward.                  (* return *)
+      destruct c' as [|ni' c'].
+      { simpl in H3. exfalso. apply H3. auto. }
+      destruct (isNodeParent n key). unfold r.
+      cancel. change_compspecs CompSpecs. cancel.
+      simpl in H4. inv H4.
+    + unfold cursor_rep.
+      Intros anc_end0. Intros idx_end0. unfold r.
+      forward.                  (* t'3=cursor->level *)
+      forward.                  (* cursor->level = t'3 -1 *)
+      { entailer!. rewrite Zlength_cons. rewrite Zsuccminusone.
+        apply partial_complete_length in H. rewrite Zlength_cons in H. rewrite Zsuccminusone in H.
+        rewrite Int.signed_repr by rep_omega.
+        rewrite Int.signed_repr by rep_omega. rep_omega. auto. }
+      forward_call(c',pc,key,r).   (* ascendtoparent(cursor,key) *)
+      * unfold cursor_rep. Exists (getval n :: anc_end0). Exists (Vint(Int.repr(rep_index i)) :: idx_end0).
+        unfold r.
+        simpl. cancel. rewrite Zlength_cons. rewrite Zsuccminusone.
+        replace (Int.sub (Int.repr (Zlength c')) (Int.repr 1)) with (Int.repr(Zlength c' - 1)).
+        rewrite <- app_assoc. rewrite <- app_assoc. simpl. cancel.
+        change_compspecs CompSpecs. cancel.
+        apply partial_complete_length in H; auto.
+        rewrite Zlength_cons in H. rewrite Zsuccminusone in H. unfold Int.sub.
+        rewrite Int.unsigned_repr by rep_omega. rewrite Int.unsigned_repr by rep_omega. auto.
+      * split. left. unfold ne_partial_cursor.
+        split.
+        { destruct H.
+          - inv H. destruct H6. simpl in H5. destruct (nth_node i n) eqn:NTH; try contradiction.
+            destruct H5. unfold partial_cursor_correct_rel.
+            destruct c'. auto. destruct p.
+            assert(CORRECT:partial_cursor_correct ((n1, i0) :: c') n root) by auto.
+            simpl in H5. destruct H5. rewrite H8. auto.
+          - inv H. unfold complete_cursor_correct_rel in H5.
+            destruct (getCEntry ((n,i)::c')); try contradiction.
+            destruct e; try contradiction.
+            simpl in H5. destruct i; try contradiction.
+            destruct H5. unfold partial_cursor_correct_rel.
+            destruct c'. auto. destruct p.
+            assert(CORRECT: partial_cursor_correct ((n1, i) :: c') n root) by auto.
+            simpl in H. destruct H. rewrite H7. auto. }
+        split. destruct c'. simpl in H3. exfalso. apply H3. auto. simpl. omega.
+        destruct H; inv H; auto. destruct H6. auto.
+        split. auto. split; auto.
+      * forward.                 (* return *)
+        destruct c' as [|ni' c''].
+        { simpl in H3. exfalso. apply H3. auto. }
+        destruct (isNodeParent n key).
+        { simpl in H4. inv H4. }
+        unfold r. cancel.
+Qed.     
+
+Lemma ne_ascend: forall (X:Type) (c:cursor X) key,
+    c <> [] -> AscendToParent c key <> [].
+Proof.
+  destruct c as [|[n i] c'].
+  - intros. exfalso. apply H. auto.
+  - intros. generalize dependent n. generalize dependent i. induction c' as [|[n0 i0] c''].
+    + simpl. auto.
+    + intros. replace (AscendToParent ((n, i) :: (n0, i0) :: c'') key) with (if (isNodeParent n key) then (n,i)::(n0,i0)::c'' else AscendToParent ((n0,i0)::c'') key).
+      destruct(isNodeParent n key).
+      * auto.
+      * apply IHc''. unfold not. intros. inv H0.
+      * simpl. auto.
+Qed.
+
+Lemma ascend_correct: forall c r key,
+    complete_cursor c r ->
+    ne_partial_cursor (AscendToParent c key) r \/ complete_cursor (AscendToParent c key) r.
+Proof.
+Admitted.
+
+Lemma partial_tl: forall (X:Type) p (c:cursor X) r,
+    partial_cursor_correct_rel (p::c) r ->
+    partial_cursor_correct_rel c r.
+Proof.
+  intros.
+Admitted.
+
+Lemma complete_tl: forall (X:Type) p (c:cursor X) r,
+    complete_cursor_correct_rel (p::c) r ->
+    partial_cursor_correct_rel c r.
+Proof.
+  intros.
 Admitted.
 
 Lemma body_goToKey: semax_body Vprog Gprog f_goToKey goToKey_spec.
 Proof.
   start_function.
-Admitted.
+  destruct r as [root prel].
+  pose (r:=(root,prel)).
+  forward_if(PROP (pc<>nullval) LOCAL (temp _cursor pc; temp _key (key_repr key))  SEP (relation_rep r; cursor_rep c r pc)).
+  - forward.                    (* skip *)
+    fold r. entailer!.
+  - assert_PROP(False). entailer!. inv H4.
+  - forward_call(c,pc,key,r).   (* ascendtoparent(cursor,key) *)
+    forward_call(r,(AscendToParent c key),pc).       (* t'1=currnode(cursor) *)
+    { split; auto. destruct c as [|[n i] c]. right. auto.
+      apply ascend_correct. auto. }
+    unfold cursor_rep. Intros anc_end. Intros idx_end. unfold r.
+    forward.                    (* t'2=cursor-level *)
+    destruct(AscendToParent c key) as [|[n i] asc'] eqn:HAS.
+    { exfalso. apply ne_ascend in HAS. auto. destruct c. inv H. inv H4. unfold not. intros. inv H4. }
+    simpl.
+    forward_call(n,key,asc',pc,r). (* movetoKey(t'1,key,cursor,t'2) *)
+    { entailer!. rewrite Zlength_cons. rewrite Zsuccminusone. auto. }
+    + unfold subcursor_rep. Exists (getval n :: anc_end).
+      Exists (Vint(Int.repr (rep_index i)) :: idx_end).
+      Exists (Zlength((n,i)::asc') -1).
+      unfold r. rewrite <- app_assoc.
+      rewrite <- app_assoc. simpl. cancel.
+      change_compspecs CompSpecs. cancel.
+    + split3; auto. apply ascend_correct with (key:=key) in H.
+      { destruct H.
+        - rewrite HAS in H. inv H. unfold partial_cursor. destruct H5. split; auto.
+          eapply partial_tl. eauto.
+        - rewrite HAS in H. inv H. unfold partial_cursor. split; auto.
+          eapply complete_tl. eauto. }          
+      split3; auto.
+      apply ascend_correct with (key:=key) in H. rewrite HAS in H.
+      destruct H.
+      * inv H. unfold partial_cursor_correct_rel in H4. destruct  (nth_node i n).
+        simpl in H4. destruct H4.
+        destruct asc'. simpl. subst. auto. simpl in H. destruct p.
+        destruct H. simpl. auto. contradiction.
+      * inv H. unfold complete_cursor_correct_rel in H4.
+        destruct(getCEntry ((n,i)::asc')); try contradiction.
+        destruct e; try contradiction. simpl in H4.
+        destruct i; try contradiction. destruct H4.
+        destruct asc'. simpl. simpl in H. subst. auto.
+        simpl. destruct p. simpl in H. destruct H. auto.
+    + forward.                  (* return *)
+      cancel. unfold goToKey. rewrite HAS. fold r. cancel.
+Qed.
+    
